CN_Lib/CN_Lib_Tactics.lean
@@ -1,5 +1,6 @@
 import Iris.Proofmode.Tactics
 import Iris.BI.Lib.Fixpoint
+import Iris.BI.Lib.GenHeap
 import Qq
 import Batteries.Tactic.SeqFocus
 import Lean.Elab
@@ -8,9 +9,9 @@ import CN_Lib.CN_Lib
 
 open Lean Elab Tactic Qq
 
--- This file contains some useful tactics for proofs involving CN ownership predicates over integer types.
-
 namespace CN_Lib
+
+-- This file contains some useful tactics for proofs involving CN ownership predicates over integer types.
 
 declare_syntax_cat ident_tuple
 scoped syntax "(" ident "," ident ")":ident_tuple
@@ -27,22 +28,25 @@ macro_rules
         own_eq $f $[$tl]*)
 
 -- Tactic that destructs owned predicates into their component Owned_UChar predicates
-scoped syntax "destruct_owned" pmTerm_tuple ident : tactic
+scoped syntax "destruct_owned" pmTerm_tuple ident ident : tactic
 macro_rules
-  | `(tactic| destruct_owned ($HOwn, $HOwn') $f) =>
+  | `(tactic| destruct_owned ($HOwn, $HOwn') $f1 $fi) =>
       `(tactic| first
         | icases $HOwn with ⟨H1, ⟨H2, ⟨H3, ⟨H4, HOwn⟩⟩⟩⟩ <;>
           icases HOwn with ⟨H5, ⟨H6, ⟨H7, ⟨H8, _⟩⟩⟩⟩ <;>
           icases $HOwn' with ⟨H1', ⟨H2', ⟨H3', ⟨H4', HOwn'⟩⟩⟩⟩ <;>
           icases HOwn' with ⟨H5', ⟨H6', ⟨H7', ⟨H8', _⟩⟩⟩⟩ <;>
-          own_eq $f (H1, H1') (H2, H2') (H3, H3') (H4, H4')
+          own_eq $f1 (H1, H1')
+          own_eq $fi (H2, H2') (H3, H3') (H4, H4')
             (H5, H5') (H6, H6') (H7, H7') (H8, H8')
         | icases $HOwn with ⟨H1, ⟨H2, ⟨H3, ⟨H4, _⟩⟩⟩⟩ <;>
           icases $HOwn' with ⟨H1', ⟨H2', ⟨H3', ⟨H4', _⟩⟩⟩⟩ <;>
-          own_eq $f (H1, H1') (H2, H2') (H3, H3') (H4, H4')
-        | icases $HOwn with ⟨H1, H2⟩ <;>
-          icases $HOwn' with ⟨H1', H2'⟩ <;>
-          own_eq $f (H1, H1') (H2, H2')
+          own_eq $f1 (H1, H1')
+          own_eq $fi (H2, H2') (H3, H3') (H4, H4')
+        | icases $HOwn with ⟨H1, ⟨H2 , _⟩⟩ <;>
+          icases $HOwn' with ⟨H1', ⟨H2' , _⟩⟩ <;>
+          own_eq $f1 (H1, H1')
+          own_eq $fi (H2, H2')
           )
 
 -- Macro that proves `f v = f v'` from `f : Fin n → Int` and seperate hypotheses stating
@@ -55,58 +59,51 @@ macro_rules
       apply Fin.elim0 <;> assumption)
 
 -- Tactic that solves goals of the form ⌜v = v'⌝ given a pair of owned signed predicates
-elab "solve_owned_eq_signed" HOwn:pmTerm_tuple f:ident
-  f_bytes:ident min:ident max:ident
-  v:ident v':ident H:ident H':ident : tactic => do
+elab "solve_owned_eq_signed"
+  f_bytes:ident f1:ident fi:ident
+  min:ident max:ident
+  v:ident v':ident : tactic => do
   evalTactic <| ← `(tactic|
-    destruct_owned $HOwn $f <;> ipureintro <;>
+    (iintro ⟨%x , ⟨%HEq , ⟨HOwn , ⟨%H , _⟩⟩⟩⟩ ⟨%x' , ⟨%HEq' , ⟨HOwn' , ⟨%H' , _⟩⟩⟩⟩) <;>
+    simp [-$f_bytes] <;>
+    (have HEq : x' = x := by simpa [HEq'] using HEq) <;> rw [HEq] <;>
+    destruct_owned (HOwn,HOwn') $f1 $fi <;> ipureintro <;>
     (have Hbytes : $f_bytes (wrapI $min $max $v) = $f_bytes (wrapI $min $max $v') := by
       solve_fin_from_cases) <;>
     have Hv := wrapI_within_bounds (x := $v) (min := $min) (max := $max) (by lia) <;>
     have Hv' := wrapI_within_bounds (x := $v') (min := $min) (max := $max) (by lia) <;>
     (first
-      | have HEq := CN_Lib.UShort_eq Hv Hv' Hbytes <;> apply wrapI_Short_cong $H $H' HEq
-      | have HEq := CN_Lib.UInt_eq Hv Hv' Hbytes <;> apply wrapI_Int_cong $H $H' HEq
-      | have HEq := CN_Lib.ULong_eq Hv Hv' Hbytes <;> apply wrapI_Long_cong $H $H' HEq)
+      | have HEq := CN_Lib.UShort_eq Hv Hv' Hbytes <;> apply wrapI_Short_cong H H' HEq
+      | have HEq := CN_Lib.UInt_eq Hv Hv' Hbytes <;> apply wrapI_Int_cong H H' HEq
+      | have HEq := CN_Lib.ULong_eq Hv Hv' Hbytes <;> apply wrapI_Long_cong H H' HEq)
     )
 
 -- Tactic that solves goals of the form ⌜v = v'⌝ given a pair of owned unsigned predicates
-elab "solve_owned_eq_unsigned" HOwn:pmTerm_tuple f:ident
-  f_bytes:ident
-  v:ident v':ident H:ident H':ident : tactic => do
+elab "solve_owned_eq_unsigned"
+  f_bytes:ident f1:ident fi:ident
+  v:ident v':ident: tactic => do
   evalTactic <| ← `(tactic|
-    destruct_owned $HOwn $f <;> ipureintro <;>
+    (iintro ⟨%x , ⟨%HEq , ⟨HOwn , ⟨%H , _⟩⟩⟩⟩ ⟨%x' , ⟨%HEq' , ⟨HOwn' , ⟨%H' , _⟩⟩⟩⟩) <;>
+    simp [-$f_bytes] <;>
+    (have HEq : x' = x := by simpa [HEq'] using HEq) <;> rw [HEq] <;>
+    destruct_owned (HOwn, HOwn') $f1 $fi <;> ipureintro <;>
     (have Hbytes : $f_bytes $v = $f_bytes $v' := by
       funext i
       repeat refine Fin.lastCases ?_ ?_ i; lia; intro i
       apply Fin.elim0; assumption) <;>
     (first
-      | have HEq := CN_Lib.ULong_eq $H $H' Hbytes <;> assumption
-      | have HEq := CN_Lib.UInt_eq $H $H' Hbytes <;> assumption
-      | have HEq := CN_Lib.UShort_eq $H $H' Hbytes <;> assumption
-      )
-    )
-
--- Tactic that tries to apply the above two tactics for each supported C integer type
-elab "solve_owned_eq" f:ident HOwn:pmTerm_tuple
-  v:ident v':ident
-  H:ident H':ident : tactic => do
-  evalTactic <| ← `(tactic|
-    (first
-      | solve_owned_eq_unsigned $HOwn $f ULong_bytes $v $v' $H $H'
-      | solve_owned_eq_unsigned $HOwn $f UInt_bytes $v $v' $H $H'
-      | solve_owned_eq_unsigned $HOwn $f UShort_bytes $v $v' $H $H'
-      | solve_owned_eq_signed $HOwn $f UInt_bytes min_UInt max_UInt $v $v' $H $H'
-      | solve_owned_eq_signed $HOwn $f UShort_bytes min_UShort max_UShort $v $v' $H $H'
-      | solve_owned_eq_signed $HOwn $f ULong_bytes min_ULong max_ULong $v $v' $H $H'
+      | have HEq := CN_Lib.ULong_eq H H' Hbytes <;> assumption
+      | have HEq := CN_Lib.UInt_eq H H' Hbytes <;> assumption
+      | have HEq := CN_Lib.UShort_eq H H' Hbytes <;> assumption
       )
     )
 
 -- Tactic that solves inequalities of the form ⌜l ≠ l'⌝ given a pair of owned predicates
 scoped syntax "solve_own_neq" ident ident: tactic
 macro_rules
-  | `(tactic| solve_own_neq $f $g) =>
-      `(tactic| unfold $f <;>
-          iintro ⟨H1 , _⟩ ⟨H2 , _⟩; simp <;>
-          icases H1 with ⟨H1 , _⟩; icases H2 with ⟨H2 , _⟩ <;>
-          iapply $g:ident $$ H1 H2)
+  | `(tactic| solve_own_neq $f1 $f2) =>
+      `(tactic| unfold $f1 $f2 <;>
+          iintro ⟨%x , ⟨%HEq , ⟨HOwn , _⟩⟩⟩ ⟨%x' , ⟨%HEq' , ⟨HOwn' , _⟩⟩⟩ <;>
+          simp <;>
+          icases HOwn with ⟨H1 , _⟩; icases HOwn' with ⟨H2 , _⟩ <;>
+          (ihave %HNeq := Iris.pointsTo_ne $$ H1 H2; ipureintro) <;> lia)
